thy/Iptables_Semantics/Primitive_Matchers/Transform.thy
@@ -748,7 +748,7 @@ theorem transform_normalize_primitives:
       for f :: "'c negation_type list \<Rightarrow> 'c list" and rs disc sel and C :: "'c \<Rightarrow> 'i::len common_primitive"
       by metis
     from preserve_normalized_src_ports[OF normalized_rs1 normalized_src_ports wf_disc_sel_common_primitive(2),
-         where f2 (* f *) = "(\<lambda>me. map (\<lambda>pt. [pt]) (ipt_ports_compress me))",
+         where f2 (* f *) = "(\<lambda>me. map (\<lambda>pt. [pt]) (raw_ports_compress me))",
          folded normalize_ports_step_def normalize_dst_ports_def]
     have normalized_src_ports_rs2: "\<forall>m \<in> get_match ` set ?rs2.  normalized_src_ports m" by force
     from preserve_normalized_src_ports[OF normalized_rs2 normalized_src_ports_rs2 wf_disc_sel_common_primitive(3),
@@ -806,11 +806,11 @@ theorem transform_normalize_primitives:
      have "\<forall>m\<in>get_match ` set ?rs0. normalized_n_primitive (disc2, sel2) f m"
       by (metis a' optimize_matches_option_compress_normalize_besteffort_preserves_unrelated_normalized_n_primitive) 
      with normalized_rs0 normalize_rules_preserves_unrelated_normalized_n_primitive[OF _ wf_disc_sel_common_primitive(1) a_Src_Ports,
-       of ?rs0 sel2 f "(\<lambda>me. map (\<lambda>pt. [pt]) (ipt_ports_compress me))",
+       of ?rs0 sel2 f "(\<lambda>me. map (\<lambda>pt. [pt]) (raw_ports_compress me))",
        folded normalize_src_ports_def normalize_ports_step_def]
      have "\<forall>m\<in>get_match ` set ?rs1. normalized_n_primitive (disc2, sel2) f m" by blast
      with normalized_rs1 normalize_rules_preserves_unrelated_normalized_n_primitive[OF _ wf_disc_sel_common_primitive(2) a_Dst_Ports,
-       of ?rs1 sel2 f "(\<lambda>me. map (\<lambda>pt. [pt]) (ipt_ports_compress me))",
+       of ?rs1 sel2 f "(\<lambda>me. map (\<lambda>pt. [pt]) (raw_ports_compress me))",
        folded normalize_dst_ports_def normalize_ports_step_def]
      have "\<forall>m\<in>get_match ` set ?rs2. normalized_n_primitive (disc2, sel2) f m" by blast
      with normalized_rs2 normalize_rules_preserves_unrelated_normalized_n_primitive[OF _ wf_disc_sel_common_primitive(3) a_Src,
@@ -884,9 +884,9 @@ theorem transform_normalize_primitives:
         apply(simp; fail)
        apply(simp; fail)
       using x[OF wf_disc_sel_common_primitive(1), 
-             of "(\<lambda>me. map (\<lambda>pt. [pt]) (ipt_ports_compress me))",folded normalize_src_ports_def normalize_ports_step_def] apply blast
+             of "(\<lambda>me. map (\<lambda>pt. [pt]) (raw_ports_compress me))",folded normalize_src_ports_def normalize_ports_step_def] apply blast
      using x[OF wf_disc_sel_common_primitive(2), 
-            of "(\<lambda>me. map (\<lambda>pt. [pt]) (ipt_ports_compress me))",folded normalize_dst_ports_def normalize_ports_step_def] apply blast
+            of "(\<lambda>me. map (\<lambda>pt. [pt]) (raw_ports_compress me))",folded normalize_dst_ports_def normalize_ports_step_def] apply blast
     using x[OF wf_disc_sel_common_primitive(3), of ipt_iprange_compress,folded normalize_src_ips_def] apply blast
    using x[OF wf_disc_sel_common_primitive(4), of ipt_iprange_compress,folded normalize_dst_ips_def] apply blast
    done
@@ -955,9 +955,9 @@ theorem transform_normalize_primitives:
         apply(simp; fail)
        apply(simp; fail)
       using x[OF wf_disc_sel_common_primitive(1), 
-             of "(\<lambda>me. map (\<lambda>pt. [pt]) (ipt_ports_compress me))",folded normalize_src_ports_def normalize_ports_step_def] apply blast
+             of "(\<lambda>me. map (\<lambda>pt. [pt]) (raw_ports_compress me))",folded normalize_src_ports_def normalize_ports_step_def] apply blast
      using x[OF wf_disc_sel_common_primitive(2), 
-            of "(\<lambda>me. map (\<lambda>pt. [pt]) (ipt_ports_compress me))",folded normalize_dst_ports_def normalize_ports_step_def] apply blast
+            of "(\<lambda>me. map (\<lambda>pt. [pt]) (raw_ports_compress me))",folded normalize_dst_ports_def normalize_ports_step_def] apply blast
     using x[OF wf_disc_sel_common_primitive(3), of ipt_iprange_compress,folded normalize_src_ips_def] apply blast
    using x[OF wf_disc_sel_common_primitive(4), of ipt_iprange_compress,folded normalize_dst_ips_def] apply blast
    done
